src/Crypto/AESEncryption.dfy
@@ -3,82 +3,88 @@
 
 include "../../libraries/src/Wrappers.dfy"
 include "../StandardLibrary/StandardLibrary.dfy"
+include "Model/Aws.Cryptography.PrimitivesAbstract.dfy"
 
 module {:extern "AESEncryption"} AESEncryption {
   import opened Wrappers
   import opened UInt = StandardLibrary.UInt
-
-  export
-    provides AESDecrypt, AESEncrypt, AESDecryptExtern, AESEncryptExtern, Wrappers,
-      UInt, PlaintextDecryptedWithAAD, EncryptionOutputEncryptedWithAAD, CiphertextGeneratedWithPlaintext,
-      EncryptedWithKey, DecryptedWithKey
-    reveals 
-      EncryptionOutput, 
-      AES_GCM,
-      KeyLength,
-      TagLength,
-      IVLength
-
-  type KeyLength = l: uint8 | l == 32 || l == 24 || l == 16 witness 32
-  type TagLength = l: uint8 | l == 16 witness 16
-  type IVLength = l: uint8 | l == 12 witness 12
-
-  datatype AES_GCM = AES_GCM(
-    nameonly keyLength: KeyLength,
-    nameonly tagLength: TagLength,
-    nameonly ivLength: IVLength
-  )
-
-  datatype EncryptionOutput = EncryptionOutput(cipherText: seq<uint8>, authTag: seq<uint8>)
+  import Types = AwsCryptographyPrimitivesTypes
 
   // The following are used to tie plaintext and ciphertext with the AAD that was used to produce them.
   // These assumptions can be used in the postconditions of externs, and be referenced elsewhere
   // in order to ensure that the AAD used is as expected.
   predicate {:axiom} PlaintextDecryptedWithAAD(plaintext: seq<uint8>, aad: seq<uint8>)
-  predicate {:axiom} EncryptionOutputEncryptedWithAAD(ciphertext: EncryptionOutput, aad: seq<uint8>)
+  predicate {:axiom} EncryptionOutputEncryptedWithAAD(output: Types.AESEncryptOutput, aad: seq<uint8>)
   predicate {:axiom} CiphertextGeneratedWithPlaintext (ciphertext: seq<uint8>, plaintext: seq<uint8>)
   predicate {:axiom} EncryptedWithKey(ciphertext: seq<uint8>, key: seq<uint8>)
   predicate {:axiom} DecryptedWithKey(key: seq<uint8>, plaintext: seq<uint8>)
 
-  function method EncryptionOutputFromByteSeq(s: seq<uint8>, encAlg: AES_GCM): (encArt: EncryptionOutput)
-    requires |s| >= encAlg.tagLength as int
+  function method EncryptionOutputFromByteSeq(s: seq<uint8>, encAlg: Types.AES_GCM): (encArt: Types.AESEncryptOutput)
+    requires 0 < encAlg.tagLength 
+    requires encAlg.tagLength as nat <= |s|
     ensures |encArt.cipherText + encArt.authTag| == |s|
     ensures |encArt.authTag| == encAlg.tagLength as int
   {
-    EncryptionOutput(s[.. |s| - encAlg.tagLength as int], s[|s| - encAlg.tagLength as int ..])
+    assert |s| - encAlg.tagLength as int <= |s|;
+
+    var cipherText := s[.. |s| - encAlg.tagLength as int];
+    var authTag := s[|s| - encAlg.tagLength as int ..];
+
+    Types.AESEncryptOutput(cipherText := cipherText, authTag := authTag)
   }
 
-  method {:extern "AESEncryption.AES_GCM", "AESEncryptExtern"} AESEncryptExtern(encAlg: AES_GCM, iv: seq<uint8>, key: seq<uint8>, msg: seq<uint8>, aad: seq<uint8>)
-      returns (res : Result<EncryptionOutput, string>)
+  method {:extern "AESEncryption.AES_GCM", "AESEncryptExtern"} AESEncryptExtern(
+    encAlg: Types.AES_GCM,
+    iv: seq<uint8>,
+    key: seq<uint8>,
+    msg: seq<uint8>,
+    aad: seq<uint8>
+  )
+    returns (res : Result<Types.AESEncryptOutput, Types.OpaqueError>)
     requires |iv| == encAlg.ivLength as int
     requires |key| == encAlg.keyLength as int
     ensures res.Success? ==> EncryptionOutputEncryptedWithAAD(res.value, aad)
     ensures res.Success? ==> CiphertextGeneratedWithPlaintext(res.value.cipherText, msg)
     ensures res.Success? ==> EncryptedWithKey(res.value.cipherText, key)
 
-  method AESEncrypt(encAlg: AES_GCM, iv: seq<uint8>, key: seq<uint8>, msg: seq<uint8>, aad: seq<uint8>)
-      returns (res : Result<EncryptionOutput, string>)
-    requires |iv| == encAlg.ivLength as int
-    requires |key| == encAlg.keyLength as int
+  method AESEncrypt(input: Types.AESEncryptInput)
+    returns (res : Result<Types.AESEncryptOutput, Types.Error>)
+    requires |input.iv| == input.encAlg.ivLength as int
+    requires |input.key| == input.encAlg.keyLength as int
     ensures res.Success? ==>
-      |res.value.cipherText| == |msg| && |res.value.authTag| == encAlg.tagLength as int
-    ensures res.Success? ==> EncryptionOutputEncryptedWithAAD(res.value, aad)
-    ensures res.Success? ==> CiphertextGeneratedWithPlaintext(res.value.cipherText, msg)
-    ensures res.Success? ==> EncryptedWithKey(res.value.cipherText, key)
+      && |res.value.cipherText| == |input.msg|
+      && |res.value.authTag| == input.encAlg.tagLength as int
+    ensures res.Success? ==> EncryptionOutputEncryptedWithAAD(res.value, input.aad)
+    ensures res.Success? ==> CiphertextGeneratedWithPlaintext(res.value.cipherText, input.msg)
+    ensures res.Success? ==> EncryptedWithKey(res.value.cipherText, input.key)
     // This is useful information to have to prove correctness
-    ensures res.Success? ==> |res.value.authTag| == encAlg.tagLength as nat
-    {
-      res := AESEncryptExtern(encAlg, iv, key, msg, aad);
-      if (res.Success? && |res.value.cipherText| != |msg|){
-        res := Failure("AESEncrypt did not return cipherText of expected length");
-      }
-      if (res.Success? && |res.value.authTag| != encAlg.tagLength as int){
-        res := Failure("AESEncryption did not return valid tag");
-      }
-    }
+    ensures res.Success? ==> |res.value.authTag| == input.encAlg.tagLength as nat
+  {
+    var AESEncryptInput(encAlg, iv, key, msg, aad) := input;
 
-  method {:extern "AESEncryption.AES_GCM", "AESDecryptExtern"} AESDecryptExtern(encAlg: AES_GCM, key: seq<uint8>, cipherTxt: seq<uint8>, authTag: seq<uint8>, iv: seq<uint8>, aad: seq<uint8>)
-      returns (res: Result<seq<uint8>, string>)
+    var value :- AESEncryptExtern(encAlg, iv, key, msg, aad);
+
+    :- Need(
+      |value.cipherText| == |msg|,
+      Types.AwsCryptographicPrimitivesError("AESEncrypt did not return cipherText of expected length")
+    );
+    :- Need(
+      |value.authTag| == encAlg.tagLength as int,
+      Types.AwsCryptographicPrimitivesError("AESEncryption did not return valid tag")
+    );
+
+    return Success(value);
+}
+
+  method {:extern "AESEncryption.AES_GCM", "AESDecryptExtern"} AESDecryptExtern(
+    encAlg: Types.AES_GCM,
+    key: seq<uint8>,
+    cipherTxt: seq<uint8>,
+    authTag: seq<uint8>,
+    iv: seq<uint8>,
+    aad: seq<uint8>
+  )
+    returns (res: Result<seq<uint8>, Types.OpaqueError>)
     requires |key| == encAlg.keyLength as int
     requires |iv| == encAlg.ivLength as int
     requires |authTag| == encAlg.tagLength as int
@@ -86,20 +92,27 @@ module {:extern "AESEncryption"} AESEncryption {
     ensures res.Success? ==> CiphertextGeneratedWithPlaintext(cipherTxt, res.value)
     ensures res.Success? ==> DecryptedWithKey(key, res.value)
 
-  method AESDecrypt(encAlg: AES_GCM, key: seq<uint8>, cipherTxt: seq<uint8>, authTag: seq<uint8>, iv: seq<uint8>, aad: seq<uint8>)
-      returns (res: Result<seq<uint8>, string>)
-    requires |key| == encAlg.keyLength as int
-    requires |iv| == encAlg.ivLength as int
-    requires |authTag| == encAlg.tagLength as int
-    ensures res.Success? ==> |res.value| == |cipherTxt|
-    ensures res.Success? ==> PlaintextDecryptedWithAAD(res.value, aad)
-    ensures res.Success? ==> CiphertextGeneratedWithPlaintext(cipherTxt, res.value)
-    ensures res.Success? ==> DecryptedWithKey(key, res.value)
-    {
-      res := AESDecryptExtern(encAlg, key, cipherTxt, authTag, iv, aad);
-      if (res.Success? && |cipherTxt| != |res.value|){
-        res := Failure("AESDecrypt did not return plaintext of expected length");
-      }
-    }
+  method AESDecrypt(
+    input: Types.AESDecryptInput
+  )
+    returns (res: Result<seq<uint8>, Types.Error>)
+    requires |input.key| == input.encAlg.keyLength as int
+    requires |input.iv| == input.encAlg.ivLength as int
+    requires |input.authTag| == input.encAlg.tagLength as int
+    ensures res.Success? ==> |res.value| == |input.cipherTxt|
+    ensures res.Success? ==> PlaintextDecryptedWithAAD(res.value, input.aad)
+    ensures res.Success? ==> CiphertextGeneratedWithPlaintext(input.cipherTxt, res.value)
+    ensures res.Success? ==> DecryptedWithKey(input.key, res.value)
+  {
+    var AESDecryptInput(encAlg, key, cipherTxt, authTag, iv, aad) := input;
+    var value :- AESDecryptExtern(encAlg, key, cipherTxt, authTag, iv, aad);
+
+    :- Need(
+      |cipherTxt| == |value|,
+      Types.AwsCryptographicPrimitivesError("AESDecrypt did not return plaintext of expected length")
+    );
+
+    return Success(value);
+  }
 
 }
