src/Crypto/Index.dfy
@@ -1,0 +1,115 @@
+// Copyright Amazon.com Inc. or its affiliates. All Rights Reserved.
+// SPDX-License-Identifier: Apache-2.0
+
+include "Model/Aws.Cryptography.PrimitivesAbstract.dfy"
+include "../StandardLibrary/StandardLibrary.dfy"
+include "Random.dfy"
+include "AESEncryption.dfy"
+include "Digest.dfy"
+// include "RSAEncryption.dfy"
+// include "Signature.dfy"
+
+// TODO add back the `Aws.`
+module Aws.Cryptography.Primitives {
+  import Random
+  import AESEncryption
+  import D = Digest
+  import opened AwsCryptographyPrimitivesTypes
+  import opened Wrappers
+  import opened StandardLibrary.UInt
+
+  class AwsCryptographicPrimitives extends IAwsCryptographicPrimitivesClient {
+
+    method CreateAtomicPrimitives ( input: AwsCryptographicPrimitivesVersion )
+      returns  ( output: Result<IAtomicPrimitives, Error> )
+      ensures CreateAtomicPrimitivesCalledWith (  input )
+      ensures output.Success? ==> CreateAtomicPrimitivesSucceededWith (  input , output.value )
+    {
+      var p := new AtomicPrimitives(input);
+      return Success(p);
+    }
+  }
+
+  class AtomicPrimitives extends IAtomicPrimitives {
+    const version: AwsCryptographicPrimitivesVersion;
+
+    constructor( version: AwsCryptographicPrimitivesVersion )
+      ensures this.version == version
+    {
+      this.version := version;
+    }
+
+
+    method GenerateRandomBytes ( input: GenerateRandomBytesInput )
+      returns  ( output: Result<seq<uint8>, Error> )
+	    ensures GenerateRandomBytesCalledWith (  input )
+	    ensures output.Success? ==> GenerateRandomBytesSucceededWith (  input , output.value )
+    {
+      output := Random.GenerateBytes(input.length);
+    }
+
+
+
+
+
+
+
+
+    method Digest ( input: DigestInput )
+      returns  ( output: Result<seq<uint8>, Error> )
+      ensures DigestCalledWith (  input )
+      ensures output.Success? ==> DigestSucceededWith (  input , output.value )
+    {
+      output := D.Digest(input);
+    }
+
+    method HMac ( input: HMacInput )
+      returns  ( output: Result<seq<uint8>, Error> )
+      ensures HMacCalledWith (  input )
+      ensures output.Success? ==> HMacSucceededWith (  input , output.value )
+    {
+
+    }
+
+    method HkdfExpand ( input: HkdfExpandInput )
+      returns  ( output: Result<seq<uint8>, Error> )
+      ensures HkdfExpandCalledWith (  input )
+      ensures output.Success? ==> HkdfExpandSucceededWith (  input , output.value )
+    {
+
+    }
+
+    method HkdfExtract ( input: HkdfExtractInput )
+      returns  ( output: Result<seq<uint8>, Error> )
+      ensures HkdfExtractCalledWith (  input )
+      ensures output.Success? ==> HkdfExtractSucceededWith (  input , output.value )
+    {
+
+    }
+
+    method AESDecrypt ( input: AESDecryptInput )
+      returns  ( output: Result<seq<uint8>, Error> )
+      ensures AESDecryptCalledWith (  input )
+      ensures output.Success? ==> AESDecryptSucceededWith (  input , output.value )
+    {
+      output := AESEncryption.AESDecrypt(input);
+    }
+
+    method Hkdf ( input: HkdfInput )
+      returns  ( output: Result<seq<uint8>, Error> )
+      ensures HkdfCalledWith (  input )
+      ensures output.Success? ==> HkdfSucceededWith (  input , output.value )
+    {
+
+    }
+
+    method AESEncrypt ( input: AESEncryptInput )
+      returns  ( output: Result<AESEncryptOutput, Error> )
+      ensures AESEncryptCalledWith (  input )
+      ensures output.Success? ==> AESEncryptSucceededWith (  input , output.value )
+      ensures output.Success? ==> AESEncryption.EncryptionOutputEncryptedWithAAD(output.value, input.aad)
+    {
+      output := AESEncryption.AESEncrypt(input);
+    }
+  }
+}
