src/Crypto/Random.dfy
@@ -2,32 +2,33 @@
 // SPDX-License-Identifier: Apache-2.0
 
 include "../StandardLibrary/StandardLibrary.dfy"
-include "../StandardLibrary/UInt.dfy"
-include "Model/Aws.Cryptography.Primitives.Exceptions.dfy"
+include "Model/Aws.Cryptography.PrimitivesAbstract.dfy"
 
 module Random {
   import opened Wrappers
   import opened UInt = StandardLibrary.UInt
   import ExternRandom
-  import Aws.Cryptography.Primitives.Exceptions
+  import Types = AwsCryptographyPrimitivesTypes
 
-  method GenerateBytes(i: int32) returns (res: Result<seq<uint8>, Exceptions.IAwsCryptographicPrimitivesException>)
+  method GenerateBytes(i: int32) returns (res: Result<seq<uint8>, Types.Error>)
     requires 0 <= i
     ensures res.Success? ==> |res.value| == i as int
   {
-    var result := ExternRandom.GenerateBytes(i);
-    if result.Success? && |result.value| != i as int {
-      var err := new Exceptions.AwsCryptographicPrimitivesError("Incorrect length from ExternRandom.");
-      return Failure(err);
-    }
-    return result;
+    var value :- ExternRandom.GenerateBytes(i);
+
+    :- Need(
+      |value| == i as int,
+      Types.AwsCryptographicPrimitivesError("Incorrect length from ExternRandom.")
+    );
+
+    return Success(value);
   }
 }
 
 module {:extern "ExternRandom"} ExternRandom {
   import opened Wrappers
   import opened UInt = StandardLibrary.UInt
-  import Aws.Cryptography.Primitives.Exceptions
+  import Types = AwsCryptographyPrimitivesTypes
 
-  method {:extern} GenerateBytes(i: int32) returns (res: Result<seq<uint8>, Exceptions.IAwsCryptographicPrimitivesException>)
+  method {:extern} GenerateBytes(i: int32) returns (res: Result<seq<uint8>, Types.OpaqueError>)
 }
